simplifying Blum assumptions

aux/permutation.ec
@@ -1,30 +1,25 @@
 pragma Goals:printall.
-require import AllCore List Distr  .
-
+require import AllCore List Distr.
 
 type permutation = int -> int.
 
 op compose : permutation -> permutation -> permutation 
   = (\o).
 op inv : permutation -> permutation.
+op mk_perm : int list -> permutation.
 
 
 op perm_d : int -> permutation distr.
 
+axiom perm_d_uni n : is_uniform (perm_d n).
+axiom perm_d_lossless : forall x, is_lossless (perm_d x).
+
+axiom perm_d_in1 p n w : p \in perm_d n => perm_eq w (range 0 n) => p \o (mk_perm w) \in perm_d n.
+axiom perm_d_in2 p n w : p \in perm_d n => perm_eq w (range 0 n) => p \o (inv (mk_perm w)) \in perm_d n.
+axiom perm_d_in3 n p : p \in perm_d n => perm_eq (map p  (range 0 n)) (range 0 n).
+axiom perm_d_in4 p n :  perm_eq p (range 0 n) => (mk_perm p) \in perm_d n.
+
 axiom inv_prop1 p n :  p \in perm_d n => p \o (inv p) = (fun x => x).
 axiom inv_prop2 p n :  p \in perm_d n => (inv p) \o p = (fun x => x). 
-
-op mk_perm_list_fun : int list -> permutation.
-
-
-axiom perm_d_uni n : is_uniform (perm_d n).
-axiom perm_d_in1 p n w : p \in perm_d n => p \o ((mk_perm_list_fun w)) \in perm_d n.
-axiom perm_d_in2 p n w : p \in perm_d n => p \o (inv (mk_perm_list_fun w)) \in perm_d n.
-axiom perm_d_in3 n p : p \in perm_d n => perm_eq (map p  (range 0 n)) (range 0 n).
-axiom invop p : perm_eq p (range 0 (size p)) => map (inv (mk_perm_list_fun p)) p = range 0 (size p).
-
-axiom perm_d_in4 p n :  perm_eq p (range 0 n) =>
-  (mk_perm_list_fun p) \in perm_d n.
-
-axiom perm_d_lossless : forall x, is_lossless (perm_d x).
+axiom inv_prop3 p : perm_eq p (range 0 (size p)) => map (inv (mk_perm p)) p = range 0 (size p).
 
